@prefix : <http://www.semanticweb.org/jioannou/ontologies/2017/2/data-topography#> .
@prefix owl: <http://www.w3.org/2002/07/owl#> .
@prefix rdf: <http://www.w3.org/1999/02/22-rdf-syntax-ns#> .
@prefix xml: <http://www.w3.org/XML/1998/namespace> .
@prefix xsd: <http://www.w3.org/2001/XMLSchema#> .
@prefix rdfs: <http://www.w3.org/2000/01/rdf-schema#> .

<http://www.semanticweb.org/jioannou/ontologies/2017/2/data-topography> a owl:Ontology ;
	rdfs:comment "The 'Data' ontology describes the concept of data classification. Data can be classfied into two main categories: Regular and Sensitive data. Each one category can be consisted further by some sub-classes that define their properties."@en .
# 
# 
# #################################################################
# #
# #    Data properties
# #
# #################################################################
# 
# 
# http://www.semanticweb.org/jioannou/ontologies/2017/2/data-topography#DataProps

:DataProps a owl:DatatypeProperty ;
	rdfs:comment "Represents the class of the Data property. Data props are consisted by the General Knowledge (RegularData) and the Sensitive Personal Data (SensitiveData)."@en .
# 
# http://www.semanticweb.org/jioannou/ontologies/2017/2/data-topography#RegularDescription

:RegularDescription a owl:DatatypeProperty ;
	rdfs:subPropertyOf :RegularProps ;
	rdfs:comment "Represents a data property of the Regular data description. Describes the regular data entry."@en .
# 
# http://www.semanticweb.org/jioannou/ontologies/2017/2/data-topography#RegularInformation

:RegularInformation a owl:DatatypeProperty ;
	rdfs:subPropertyOf :RegularProps ;
	rdfs:comment "Represents a data property of the Regular data information. Defines the Regular information of the specific data entry."@en .
# 
# http://www.semanticweb.org/jioannou/ontologies/2017/2/data-topography#RegularProps

:RegularProps a owl:DatatypeProperty ;
	rdfs:subPropertyOf :DataProps ;
	rdfs:comment "Represents a data property of the Regular data."@en .
# 
# http://www.semanticweb.org/jioannou/ontologies/2017/2/data-topography#RegularTopic

:RegularTopic a owl:DatatypeProperty ;
	rdfs:subPropertyOf :RegularProps ;
	rdfs:comment "Represents a data property of the Regular data topic. Defines the Regular data entry."@en .
# 
# http://www.semanticweb.org/jioannou/ontologies/2017/2/data-topography#SensitiveDescription

:SensitiveDescription a owl:DatatypeProperty ;
	rdfs:subPropertyOf :SensitiveProps ;
	rdfs:comment "Represents a data property of the sensitive data description. Describes the sensitive data entry."@en .
# 
# http://www.semanticweb.org/jioannou/ontologies/2017/2/data-topography#SensitiveInformation

:SensitiveInformation a owl:DatatypeProperty ;
	rdfs:subPropertyOf :SensitiveProps ;
	rdfs:comment "Represents a data property of the sensitive data information. Defines the sensitive information of the specific data entry."@en .
# 
# http://www.semanticweb.org/jioannou/ontologies/2017/2/data-topography#SensitiveProps

:SensitiveProps a owl:DatatypeProperty ;
	rdfs:subPropertyOf :DataProps ;
	rdfs:comment "Represents a data property of the sensitive data."@en .
# 
# http://www.semanticweb.org/jioannou/ontologies/2017/2/data-topography#SensitiveTopic

:SensitiveTopic a owl:DatatypeProperty ;
	rdfs:subPropertyOf :SensitiveProps ;
	rdfs:comment "Represents a data property of the sensitive data topic. Defines the sensitive data entry."@en .
# 
# 
# 
# #################################################################
# #
# #    Classes
# #
# #################################################################
# 
# 
# http://www.semanticweb.org/jioannou/ontologies/2017/2/data-topography#Data

:Data a owl:Class ;
	rdfs:comment "Represents the class of the Data. Data is consisted by the General Knowledge (RegularData) and the Sensitive Personal Data (SensitiveData)."@en .
# 
# http://www.semanticweb.org/jioannou/ontologies/2017/2/data-topography#RegularData

:RegularData a owl:Class ;
	rdfs:subClassOf :Data ;
	rdfs:comment "Represents the class of the Regular Data."@en .
# 
# http://www.semanticweb.org/jioannou/ontologies/2017/2/data-topography#SensitiveData

:SensitiveData a owl:Class ;
	rdfs:subClassOf :Data ;
	rdfs:comment "Represents the class of the Sensitive Data."@en .
# 
# Generated by the OWL API (version 4.2.6.20160910-2108) https://github.com/owlcs/owlapi
